misc-verification/doubly_linked_list.v
@@ -8,22 +8,38 @@
 From iris.proofmode Require Import proofmode.
 From iris.heap_lang Require Import lang proofmode notation.
 
+(*is list is empty the back pointer is last pointer (circular)*)
+(*if the list is not empty back pointer is previous to last pointer*)
+(*if the list is not empty the first element previous pointer is last pointer*)
+(*so prev/back = last is null basically*)
+(*first had null as head pointer, but push_back gets annoying, 
+   since you need to prove that if lback != lh then 
+   vs is not empty, this is true but annoying to prove 
+   now with circularity we can implement push_back without 
+   that if statement*)
+(* last pointer changes in push back still and issue so 
+tail is even better, since we can still do the trick but it is stable*)
 Definition new_list : val := λ: "_", 
-  let: "node" := Alloc (InjLV #()) in
+  (*let: "node" := Alloc NONE in*)
+  let: "node" := Alloc (InjL NONE) in
   let: "hd" := Alloc "node" in
   let: "tl" := Alloc "node" in
-  "node" <- InjL "hd";;
+  (*"node" <- InjL "node" ;;*)
   ("hd", "tl").
 
 Definition push_front : val := λ: "l" "x",
   let: "hd" := Fst "l" in
-  let: "node" := Alloc (InjR ("x", ("hd", !"hd"))) in
+  let: "tl" := Snd "l" in
+  (*tail pointer as previous -> basically our null*)
+  (*let: "node" := Alloc (InjR ("x", (!"tl", !"hd"))) in*)
+  let: "node" := Alloc (InjR ("x", (NONE, !"hd"))) in
   (*update previous pointer of next node to (current) node*)
   match: ! !"hd" with
-    InjL "lback" => !"hd" <- InjL "node"
+    InjL "lback" => !"hd" <- InjL "node" 
   | InjR "nnode" => 
       (*copy next and value over, replace previous with node*)
-      !"hd" <- InjR (Fst "nnode", ("node", Snd (Snd "nnode")))
+      (*!"hd" <- InjR (Fst "nnode", ("node", Snd (Snd "nnode")))*)
+      !"hd" <- InjR (Fst "nnode", (SOME "node", Snd (Snd "nnode")))
   end ;;
   "hd" <- "node";;
   #().
@@ -52,12 +68,8 @@ Definition push_back : val := λ: "l" "x",
   let: "tl" := Snd "l" in
   match: ! !"tl" with 
     InjL "lback" => 
-      (*lback can also be hd, then we have empty list then we just push front*)
-      if: "lback" = "hd" 
-      then push_front "l" "x"
-      else 
         match: !"lback" with 
-          InjL "_" => InjL #() (*error state, should never happen*)
+          InjL "_" => push_front "l" "x" (*we get here if lback = tl, empty list case*) 
         | InjR "pnode" => 
           let: "lnewlast" := Alloc (InjL #()) in (*() is dummy value, like in new_list*)
           let: "lnowlast" := !"tl" in
@@ -78,23 +90,18 @@ Definition pop_back : val := λ: "l", "l".
 Section Hoare.
 Context `{!heapGS_gen hlc Σ}.
 
-Implicit Types l : loc.
+Implicit Types l lh lt lstart lnext llast lback lnl : loc.
 Implicit Types v w li : val.
 
-(*not going to work for push_back and pop_back*)
 Fixpoint is_list_nodes (lprev lnow llast lback : loc) (vs : list val) : iProp Σ := 
   match vs with 
-  | [ ] => ⌜lnow = llast⌝ ∗ ⌜lprev = lback⌝
-  | [v] => lnow ↦ InjRV (v, (#lprev, (LitV (LitLoc llast)))) ∗ ⌜lnow = lback⌝
-  | v::vs => ∃ lnext, lnow ↦ InjRV (v, (#lprev, (LitV (LitLoc lnext)))) ∗ 
-                  is_list_nodes lnow lnext llast lback vs
+  | [] => ⌜lnow = llast⌝ ∗ ⌜lprev = lback⌝ 
+  | v::vs => ∃ l, lnow ↦ InjRV (v, (#lprev, #l)) ∗ is_list_nodes lnow l llast lback vs
   end.
 
 Definition is_list (v : val) (vs : list val) : iProp Σ := 
-  ∃ lh lt lnext llast, ⌜v = PairV (LitV (LitLoc lh)) (LitV (LitLoc lt))⌝ ∗ 
-    lh ↦ (LitV (LitLoc lnext)) ∗ lt ↦ (LitV (LitLoc llast)) ∗ 
-    ∃ lback, llast ↦ InjLV (LitV (LitLoc lback)) ∗ is_list_nodes lh lnext llast lback vs.
-(* see note on this *)
+  ∃ lh lt lstart llast lback, ⌜v = PairV #lh #lt⌝ ∗ lh ↦ #lstart ∗ lt ↦ #llast ∗ 
+    llast ↦ InjLV #lback ∗ is_list_nodes lt lstart llast lback vs.
      
 Lemma new_list_hoare :
   {{{ True }}}
@@ -102,8 +109,8 @@ Lemma new_list_hoare :
   {{{ vret, RET vret; is_list vret [] }}}.
 Proof. 
   iIntros "%Phi %Ht Hl". iUnfold new_list. wp_pures. wp_alloc l. wp_pures.
-  wp_alloc l'. wp_pures. wp_alloc l''. wp_store. wp_pures. iApply "Hl".
-  iUnfold is_list. iExists l', l''. by iFrame.
+  wp_alloc l'. wp_pures. wp_alloc l''. wp_pures. wp_store. wp_pures. iApply "Hl".
+  iUnfold is_list. iExists l', l'', l, l. by iFrame.
 Qed.
 
 Lemma push_front_hoare li vs v :
@@ -112,16 +119,13 @@ Lemma push_front_hoare li vs v :
   {{{ RET #(); is_list li (v :: vs) }}}.
 Proof.
   iIntros "%Phi Hisl Hl". iUnfold push_front. wp_pures. 
-  iDestruct "Hisl" as "(%lh & %lt & %ln & %ll & -> & Hlh & Hlt & %lb & Hll & Hisln)".
-  wp_load. wp_alloc lnode. wp_load. destruct vs.
+  iDestruct "Hisl" as "(%lh & %lt & %ls & %ll & %lb & -> & Hlh & Hlt & Hll & Hisln)".
+  wp_load. wp_alloc lnode as "Hlnode". wp_load. destruct vs.
   { iDestruct "Hisln" as "(<- & <-)". wp_load. wp_load. wp_store. wp_store. 
-    iApply "Hl". iUnfold is_list. iExists lh, lt, lnode, ln. by iFrame. }
-  destruct vs. 
-  { iDestruct "Hisln" as "(Hln & ->)". wp_load. wp_load. wp_store. wp_store. 
-    iApply "Hl". iUnfold is_list. iExists lh, lt, lnode, ll. by iFrame. }
-  iDestruct "Hisln" as "(%lnext & Hln & Hisnl)". fold is_list_nodes.
+    iApply "Hl". iUnfold is_list. iExists lh, lt, lnode, ls, lnode. by iFrame. }
+  iDestruct "Hisln" as "(%ln & Hln & Hisln)". fold is_list_nodes.
   wp_load. wp_load. wp_store. wp_store. iApply "Hl". iUnfold is_list.
-  iExists lh, lt, lnode, ll. by iFrame.
+  iExists lh, lt, lnode, ll, lb. by iFrame.
 Qed. 
 
 Lemma pop_front_hoare_nil li :
@@ -130,9 +134,9 @@ Lemma pop_front_hoare_nil li :
   {{{ RET InjLV #(); is_list li [] }}}.
 Proof. 
   iIntros "%Phi Hisl Hl".
-  iDestruct "Hisl" as "(%lh & %lt & %ln & %ll & -> & Hlh & Hlt & %lb & Hl2 & <- & <-)".
+  iDestruct "Hisl" as "(%lh & %lt & %ls & %ll & %lb & -> & Hlh & Hlt & Hll & (<- & <-))".
   iUnfold pop_front. wp_load. wp_load. wp_pures. iApply "Hl".
-  iUnfold is_list, is_list_nodes. iExists lh, lt, ln, ln. by iFrame.
+  iUnfold is_list, is_list_nodes. iExists lh, lt. by iFrame.
 Qed.
 
 Lemma pop_front_hoare_cons li vs v :
@@ -141,44 +145,66 @@ Lemma pop_front_hoare_cons li vs v :
   {{{ RET (InjRV v); is_list li vs }}}.
 Proof.
   iIntros "%Phi Hisl Hl".
-  iDestruct "Hisl" as "(%lh & %lt & %ln & %ll & -> & Hlh & Hlt & Hisln) /=".
-  iDestruct "Hisln" as "(%lb & Hll & Hisln)". iUnfold pop_front.
+  iDestruct "Hisl" as "(%lh & %lt & %ls & %ll & %lb & -> & Hlh & Hlt & Hll & Hisln) /=".
+  iDestruct "Hisln" as "(%ln & Hls & Hisln)". iUnfold pop_front.
   wp_load. destruct vs. 
-  { iDestruct "Hisln" as "(Hln & <-)". wp_load. wp_load. wp_free. wp_store. wp_load.
+  { iDestruct "Hisln" as "(<- & <-)". wp_load. wp_load. wp_free. wp_store. wp_load.
     wp_store. wp_pures. iApply "Hl". iUnfold is_list, is_list_nodes. 
-    iExists lh, lt, ll, ll. by iFrame. }
-  iDestruct "Hisln" as "(%lnext & Hln & Hisln)".
-  wp_load. wp_load. wp_free. wp_store. destruct vs.
-  { iDestruct "Hisln" as "(Hlnext & <-)". wp_load. wp_store. wp_pures. iApply "Hl".
-    iUnfold is_list, is_list_nodes. iExists lh, lt, lnext, ll. by iFrame. }
-  iDestruct "Hisln" as "(%lnext2 & Hlnext & Hisln)". fold is_list_nodes. 
-  wp_load. wp_store. wp_pures. iApply "Hl". 
-  iUnfold is_list, is_list_nodes. iExists lh, lt, lnext, ll. by iFrame.
+    iExists lh, lt. by iFrame. }
+  iDestruct "Hisln" as "(%ln2 & Hln & Hisln)". fold is_list_nodes.
+  wp_load. wp_load. wp_free. wp_store. wp_load. wp_store.
+  wp_pures. iApply "Hl". iUnfold is_list, is_list_nodes. 
+  iExists lh, lt, ln, ll, lb. by iFrame.
 Qed.
 
-(*stuck in proof*)
+Lemma back_pointsto_last_node lp ls ll lb vs : 
+  is_list_nodes lp ls ll lb vs -∗ 
+    match vs with 
+    | [] => is_list_nodes lp ls ll lb vs 
+    | _ => ∃ v (lp2 : loc), lb ↦ InjRV (v, (#lp2, #ll)) ∗ 
+              (lb ↦ InjRV (v, (#lp2, #ll)) -∗ is_list_nodes lp ls ll lb vs)
+    end.
+Proof.
+  iInduction vs as [|v vs IH] forall (lp ls ll lb); simpl; [done|]. 
+  iIntros "(%ln & Hls & Hisln)". iSpecialize ("IH" with "Hisln").
+  destruct vs.
+  { iDestruct "IH" as "(<- & <-)" . iExists v, lp. iSplitL "Hls"; [done|].
+    iIntros "Hls". iExists ln. iSplitL "Hls"; done. }
+  iDestruct "IH" as "(%v1 & %lp2 & Hlb & Hrec)". 
+  iExists v1, lp2. iSplitL "Hlb"; [done|]. iIntros "Hlb". iExists ln. 
+  iSplitL "Hls"; [done|]. iApply "Hrec". done.
+Qed.
+
+Lemma extend_is_list_nodes ls ll0 ll lnl lb v vs : 
+  is_list_nodes ll0 ls ll lb vs -∗ ll ↦ InjRV (v, (#lb, #lnl)) -∗ 
+    is_list_nodes ll0 ls lnl ll (vs ++ [v]).
+Proof.
+  iInduction vs as [|v' vs IH] forall (ls ll0 ll lnl lb v); simpl.
+  { iIntros "(<- & <-) Hll". by iFrame. }
+  iIntros "(%l & Hls & Hisln) Hll". iExists l. iSplitL "Hls"; [done|].
+  iApply ("IH" with "Hisln"). done.
+Qed.
+
 Lemma push_back_hoare li vs v :
   {{{ is_list li vs }}}
     push_back li v
   {{{ RET #(); is_list li (vs ++ [v]) }}}.
 Proof.
   iIntros "%Phi Hisl Hl". 
-  iDestruct "Hisl" as "(%lh & %lt & %ln & %ll & -> & Hlh & Hlt & %lb & Hll & Hisln)".
-  iUnfold push_back. wp_load. wp_load. wp_pures. destruct vs.
-  { iDestruct "Hisln" as "(<- & <-)". destruct (bool_decide (#lh = #lh)) eqn:Heq. wp_pures.
-    - iApply ((push_front_hoare (LitV (LitLoc lh), LitV (LitLoc lt)) [] v) 
-      with "[Hlh Hlt Hll] [Hl]"); simpl; [|iApply "Hl"].
-      iUnfold is_list, is_list_nodes. iExists lh, lt, ln, ln. by iFrame.
-    - admit. (*should be easy*) }
-  destruct (bool_decide (#lb = #lh)) eqn:Heq.
-  { admit. (*need to prove that lb != lh if not empty :|, seems tediouss,
-      should get it from seperation logic but how?*) }
-  wp_pures. destruct vs.
-  { iDestruct "Hisln" as "(Hlnext & <-)". wp_load. wp_alloc lnewlast. wp_load. 
-    wp_store. wp_store. wp_store. wp_store. iApply "Hl". iUnfold is_list.
-    iExists lh, lt, ln, lnewlast. by iFrame. }
-  iDestruct "Hisln" as "(%lnext2 & Hlnext & Hisln)". fold is_list_nodes. 
-  wp_load.
+  iDestruct "Hisl" as "(%lh & %lt & %ls & %ll & %lb & -> & Hlh & Hlt & Hll & Hisln)".
+  iUnfold push_back. wp_load. wp_load. wp_pures. 
+  iPoseProof (back_pointsto_last_node with "Hisln") as "Hlb";
+  destruct vs.
+  { iDestruct "Hlb" as "(<- & <-)". wp_load. wp_load. wp_pures.
+    iApply ((push_front_hoare (#lh, #lt) [] v) with "[Hlh Hlt Hll] [Hl]"); 
+    simpl; [|iApply "Hl"]. iUnfold is_list, is_list_nodes. iExists lh, lt. by iFrame. }
+  iDestruct "Hlb" as "(%v1 & %lp2 & Hlb & Hrec)". wp_load. wp_load.
+  wp_alloc lnl as "Hlnl". wp_load. wp_store. wp_store. wp_store. wp_store.
+  iApply "Hl". iUnfold is_list. iExists lh, lt, ls, lnl. iFrame.
+  iSplitR; [done|]. iSpecialize ("Hrec" with "Hlb").
+  iApply (extend_is_list_nodes with "[Hrec]"); [|iApply "Hll"].
+  (*ll is not stable -> lnl so maybe store tl, is stable and still can 
+     do trick in push_back*)
 Qed.
 
 End Hoare.
